csdl.v
@@ -3,15 +3,33 @@ Require Import CSDL.Basics CSDL.Binary String.
 
 Definition ty := nat.
 Definition const := bits.
-Variable operator : list ty -> ty -> Set.
 
+Fixpoint type_of_op (l : list ty) (t : ty) :=
+  match l with
+    | nil => const t
+    | t' :: l' => const t' -> type_of_op l' t
+  end.
+
+Inductive operator (l : list ty) (t : ty) : Set :=
+| OP (op : type_of_op l t).
+  
 (* Class Operator (A : Type) (a : A) := *)
 (*   { args : list ty ; *)
 (*     res *)
 
 Inductive endianness := BigEndian | LittleEndian.
 
-Variable space : Π (number : option nat) (addressing : ty) (size : ty), Set.
+Record space := mkSpace {
+  space_n : option nat;
+  space_address : ty;
+  space_cell_size : ty;
+  space_cell_size_pos : Have (space_cell_size > 0)
+}.
+
+Existing Instance space_cell_size_pos.
+  
+(* Variable space : Π (number : option nat) (addressing : ty) (size : ty), Set. *)
+
 Inductive loc (n : ty) : Set := LOC (b : bits n).
 
 Variable cells : nat -> Set. 
@@ -38,10 +56,16 @@ with args : list ty -> Set :=
 | ARGcons {ty tys} : exp ty -> args tys -> args (ty :: tys)
 
 with location : ty -> Set :=
-| AGG {n w} (b : endianness) (c : cell n) `{wgtn : Have (w > n)} `{wmultn : Have (modulo_nat w n = 0)} : location w
+| AGG {w} (b : endianness) (s : space) (e : exp s.(space_address))
+  `{wgtn : Have (w > s.(space_cell_size))}
+  `{wmultn : Have (modulo_nat w s.(space_cell_size) = 0)} : location w.
 
-with cell : ty -> Set :=
-| CELL {n a m} (s : space n a m) (e : exp a) : cell m.
+(* with location : ty -> Set := *)
+(* | AGG {n w} (b : endianness) (c : cell n) `{wgtn : Have (w > n)} `{Have (n > 0)} *)
+(*   `{wmultn : Have (modulo_nat w n = 0)} : location w *)
+
+(* with cell : ty -> Set := *)
+(* | CELL (s : space) (e : exp s.(space_address)) : cell s.(space_cell_size). *)
 
 Inductive effect : Set :=
 | STORE {n} (dst : location n) (src : exp n)
@@ -54,11 +78,11 @@ Inductive rtl := RTL (l : list guarded).
 
 Definition cell_name := string.
 
-Definition space_descr (locations : ty) (size : ty) :=
-  forall (t : ty), const locations -> option (bits t).
+Definition space_descr (sp : space) :=
+  const sp.(space_address) -> forall agg : nat, option (bits (agg * sp.(space_cell_size))).
 
-Record mem := {
-  mem_cell_fetches: forall {n a m} (sp : space n a m), space_descr a m
+Record mem := mkMem {
+  mem_cell_fetches: forall (sp : space), space_descr sp
 }.
 
 Definition interpM a := mem -> (option a * mem)%type.
@@ -74,43 +98,223 @@ Definition bind {A B} (x : interpM A) (y : A -> interpM B) : interpM B :=
 
 Axiom cheat : Π {α}, α.
 
+Definition binary_plus {n} (x y : bits n) : bits n * overflow.
+Admitted.
+Print mult.
+(* Program Fixpoint mem_cell_fetch_q (sp : space) (e : const (space_address sp)) (offset : nat) (m : mem) :  *)
+(*   option (const (offset * space_cell_size sp)) := *)
+(*   mem_cell_fetches m sp e offset.   *)
+
+
+(*   match offset return option (bits (S offset * space_cell_size sp)) with *)
+(*     | 0 => Nonemem_cell_fetches m sp e *)
+(*     | S n =>  *)
+(*       vector_append (mem_cell_fetch_q sp e n m) (mem_cell_fetches m sp (binary_plus e (space_cell_size sp))) *)
+(*   end. *)
+
+Theorem euclid_unique : 
+ forall a b `(Have (b > 0)) q r, q > r -> a = b * q + r -> r = modulo_nat a b.
+Admitted.
+
+Lemma quotient_cancel : forall x y `{Have (y > 0)}, modulo_nat x y = 0 -> quotient_nat x y * y = x.
+Admitted.
+(* Proof. intros. unfold quotient_nat.  *)
+(*   unfold modulo_nat in H0. destruct_call modulo. *)
+(*   simpl in *. subst. *)
+(*   destruct e as [q [ Hq Hy'] ]. *)
+(*   pose (euclid_unique x y H q 0). *)
+
+Require Import Le.
+Definition ltb (x y : nat) := leb (S x) y.
+
+Program Fixpoint euclid (n : nat) (m : nat) `{Have (m > 0)} {wf lt n} : nat * nat :=
+  match ltb n m with
+    | true => (0, n)
+    | false => let '(q, r) := euclid (n - m) m in
+      (S q, r)
+  end.
+
+Lemma minus_n_n n : n - n = 0. 
+Proof. induction n; simpl; auto. Defined.
+
+Lemma minus_n_O n : n - O = n. 
+Proof. induction n; simpl; auto. Defined.
+
+Lemma lt_n_S_n n : n < S n.
+Proof. induction n; simpl; auto. Defined.
+
+Lemma lt_trans n m p : n < m -> m < p -> n < p.
+Proof. induction 1; simpl; intros. induction H ; auto. 
+  apply IHle. inversion H0.
+
+
+
+Print Opaque Dependencies minus_n_n. 
+
+  Next Obligation.
+    unfold ltb in *.
+    symmetry in Heq_anonymous.
+    simpl in Heq_anonymous. destruct m. inversion H.
+    clear euclid. unfold Have in *.
+    clear H.
+    revert m Heq_anonymous. induction n; simpl in *; intros. discriminate.
+    destruct m. rewrite minus_n_O. constructor.
+    pose (IHn m Heq_anonymous). 
+    
+
+    Print leb_complete_conv.
+    apply leb_complete_conv in Heq_anonymous. omega. 
+  Defined.
+
+  Next Obligation. auto with *. Defined.
+
+(* induction Heq_anonymous. rewrite minus_n_n. *)
+(*     red. induction m ; simpl ; auto. *)
+(*     simpl. clear. induction m; simpl. *)
+    
+(*     constructor. *)
+(*     inversion H. si *)
+
+Eval lazy beta delta iota zeta in (euclid 8 2).
+
+Definition mem_cell_fetches_agg {w} (m : mem) (e : endianness) (sp : space) (e : const sp.(space_address)) 
+  `(wgtn : Have (w > sp.(space_cell_size))) `(Have (sp.(space_cell_size) > 0)) 
+  `(wmultn : Have (modulo_nat w sp.(space_cell_size) = 0)) : 
+  option (const w).
+  intros.
+  pose (fetch := mem_cell_fetches m sp).
+  unfold space_descr in fetch.
+  set (q := quotient_nat w (space_cell_size sp)).
+  pose (fetch e0 q).
+  subst q. rewrite quotient_cancel in o. exact o.
+  assumption.
+Defined.
+
+(* Equations mem_cell_fetches_agg {w} (e : endianness) (sp : space) (e : const sp.(space_address)) *)
+(*   `(wgtn : Have (w > sp.(space_cell_size)))  *)
+(*   `(cellgt0 : Have (sp.(space_cell_size) > 0)) *)
+(*   `(wmultn : Have (modulo_nat w sp.(space_cell_size) = 0)) : *)
+(*   option (const w) := *)
+(* mem_cell_fetches_agg w endian sp e wgtn spgt0 wmultn := *)
+
+(* Definition mem_cell_fetches_agg {n w} (e : endianness) (sp : space) (e : exp sp.(space_address))  *)
+(*   `(wgtn : Have (w > n)) `(wmultn : Have (modulo_nat w n = 0)) : option (const n) := *)
+  
 Fixpoint eval_fetch {n} (l : location n) : interpM (const n) :=
-  match l with
-    AGG n w endian (CELL num addr n' sp e) wgtn wmultn =>
-    bind (eval_exp e) (fun (c : const addr) mem =>
-      (mem_cell_fetches mem sp w c, mem))
+  match l in location n return interpM (const n) with
+    | AGG w endian sp e wgtn wmultn =>
+      bind (eval_exp e) (fun (c : const sp.(space_address)) mem =>
+        (mem_cell_fetches_agg mem endian sp c wgtn _ wmultn, mem))
   end
 
 with eval_exp {n} (e : exp n) : interpM (const n) :=
   match e with
     | CONST n c => ret c
     | FETCH n l => eval_fetch l
-    | APP l n o args => 
-      fix aux (args : args l) (op :  :=
-      match args with
-        | ARGnil => 
-| ARGcons {ty tys} : exp ty -> args tys -> args (ty :: tys)
-      map (eval_exp 
-
+    | APP l n o es => 
+      let 'OP f := o in
+        (fix aux l (es : args l) : type_of_op l n -> interpM (const n) :=
+          match es in args l return type_of_op l n -> interpM (const n) with
+            | ARGnil => fun op => ret op
+            | ARGcons ty tys e es => fun op => 
+              bind (eval_exp e) (fun e' =>
+                aux tys es (op e'))
+          end) l es f
   end.
+
+Definition eval_app {n : ty} {l : list ty} (es : args l) : type_of_op l n -> interpM (const n) :=
+  (fix aux l (es : args l) : type_of_op l n -> interpM (const n) :=
+  match es in args l return type_of_op l n -> interpM (const n) with
+    | ARGnil => fun op => ret op
+    | ARGcons ty tys e es => fun op => 
+      bind (eval_exp e) (fun e' => aux tys es (op e'))
+  end) l es.
+
+Lemma eval_exp_const n (c : const n) : eval_exp (CONST c) = ret c.
+Proof. trivial. Qed.
+
+Lemma eval_exp_fetch n (l : location n) : eval_exp (FETCH l) = eval_fetch l.
+Proof. trivial. Qed.
+
+Lemma eval_fetch_agg {w} (endian : endianness) (sp : space) e wgtn wmultn :
+  eval_fetch (@AGG w endian sp e wgtn wmultn) =
+  bind (eval_exp e) (fun (c : const sp.(space_address)) mem =>
+    (mem_cell_fetches_agg mem endian sp c wgtn _ wmultn, mem)).
+Proof. trivial. Qed.
+
+Lemma eval_exp_app {l : list ty} {n : ty} (o : type_of_op l n) (es : args l) :
+  eval_exp (APP (OP l n o) es) = eval_app es o.
+Proof. intros. simpl. unfold eval_app. trivial. Qed.
+
+Lemma eval_app_nil {n : ty} (o : type_of_op nil n) : eval_app ARGnil o = ret o.
+Proof. intros. trivial. Qed.
+
+Lemma eval_app_cons {t : ty} {l : list ty} (e : exp t) (es : args l) {n : ty} (o : type_of_op (t :: l) n) : 
+  eval_app (ARGcons e es) o = bind (eval_exp e) (fun e' => eval_app es (o e')).
+Proof. intros. trivial. Qed.
+
+
+
 
 (* Equations(nocomp) eval_fetch {n} (l : location n) : interpM (const n) := *)
 (* eval_fetch w (AGG n w e (CELL num addr n sp e) wgtn wmultn) := *)
 (*   bind (eval_exp e) (fun (c : const addr) mem => *)
 (*     (mem_cell_fetches mem sp c w, mem)). *)
 
-Equations(nocomp) eval_exp {n} (e : exp n) : interpM (const n) :=
-eval_exp n (CONST n c) := ret c ;
-eval_exp n (FETCH n l) := fetch l ;
-eval_exp n (APP l n o args) := cheat.
+(* Equations(nocomp) eval_exp {n} (e : exp n) : interpM (const n) := *)
+(* eval_exp n (CONST n c) := ret c ; *)
+(* eval_exp n (FETCH n l) := fetch l ; *)
+(* eval_exp n (APP l n o args) := cheat. *)
+
+Equations(nocomp) binary_eq {n} (x y : const n) : bool :=
+binary_eq ?(0) Vnil Vnil := true ;
+binary_eq ?(S n) (Vcons a n x) (Vcons b n y) := bool_eq a b && binary_eq x y.
+
+(* Equations(nocomp) binary_eq {n} (x y : const n) : { x = y } + { x <> y } := *)
+(* binary_eq ?(0) Vnil Vnil := left eq_refl ; *)
+(* binary_eq ?(S n) (Vcons true n x) (Vcons true n y) := if binary_eq x y then in_left else in_right ; *)
+(* binary_eq ?(S n) (Vcons false n x) (Vcons false n y) := if binary_eq x y then in_left else in_right ; *)
+(* binary_eq ?(S n) (Vcons a n _) (Vcons b n _) := in_right. *)
+
+About mem_cell_fetches. Print space_descr.
+
+Definition coerce_bits {n m} (c : bits n) (H : n = m) : bits m.
+intros ; subst. exact c. Defined.
+
+Equations mem_cell_update (m : mem) {n a w} (sp : space n a w) (e : const a) (c : const w) : mem :=
+mem_cell_update (mkMem m) n a w sp e c := 
+  let mem' n' a' w' (sp' : space n' a' w') (t : ty) (e' : const a') := 
+    if eq_nat_dec a a' then
+      if binary_eq e (coerce_bits e' _) then 
+        Some (coerce_bits c _)
+      else None
+    else m n' a' w' sp' t e' in mkMem mem'.
+
+  Next Obligation. Defined.
+  Next Obligation.   Defined.
 
   
+Equations eval_store {n} (l : location n) (c : const n) : interpM () :=
+eval_store n (AGG n w endian (CELL num a w sp e) wgtn wmultn) := 
+  bind (eval_exp e) (fun e' : const a =>
+    fun mem => ((), mem_cell_update mem sp e' c))
+  
 
+Equations(nocomp) apply_effect (e : effect) : interpM () := 
+apply_effect (STORE n dst src) :=
+  bind (eval_exp src) (fun e' => eval_store dst (Some e')) ;
+apply_effect (KILL n l) := eval_store l None.
+
+Definition one_binary_le {n : nat} : const n := 
+  fst (bits_succ _ (constant_vector n false)).
+    
 Definition one_guarded (g : guarded) : interpM () :=
   let 'GUARD n e ef := g in
-    if eval_exp e = true then
-      apply_effect ef
-    else ret ().
+    bind (eval_exp e) 
+    (fun e' => 
+      if binary_eq e' one_binary_le then
+        apply_effect ef
+       else ret ()).
 
 
 
